add a catch all clause to match

Core/Examples/Maybe.lean
@@ -8,10 +8,12 @@ import Core.Infer
 
 def c1  := match! #0 v[ g#"Nothing" •[t#0] , g#"Just" •[t#0] ]
                      v[ g#"True" , λ[t#0] g#"False" ]
+                     g#"False"
 
 def c2 := λ[t#0] match! #1
               v[ g#"Nothing" •[t#0], g#"Just" •[t#0]]
               v[ g#"False", λ[t#0] ((((g#"eq" •[ t#0 ]) •(.open) #4) • #1) •#0) ]
+              g#"False"
 
 def MaybeBoolCtx : List Global := [
 
@@ -34,6 +36,7 @@ def MaybeBoolCtx : List Global := [
         (Λ[★] λ[gt#"Eq" • t#0] λ[ gt#"Maybe" • t#0] λ[gt#"Maybe" • t#0]
           match! #1 v[ g#"Nothing" •[t#0] , g#"Just"•[t#0] ]
                     v[ c1 , c2 ]
+                    g#"False"
 
         ),
 
@@ -57,9 +60,10 @@ def MaybeBoolCtx : List Global := [
     (λ[ .global "Bool" ] λ[ .global "Bool" ]
       match! #1
       v[ g#"True", g#"False" ]
-      v[ match! #0 v[ g#"True", g#"False" ] v[ g#"True", g#"False"] ,
-         match! #0 v[ g#"True", g#"False" ] v[ g# "False", g# "False"]
-       ]),
+      v[ match! #0 v[ g#"True", g#"False" ] v[ g#"True", g#"False"] g#"False" ,
+         match! #0 v[ g#"True", g#"False" ] v[ g# "False", g# "False"] g#"False"]
+      g#"False"
+    ),
 
   -- EqBool : ∀ t. t ~ Bool → Eq t
   .instty "EqBool" (∀[★] (t#0 ~[★]~ gt#"Bool") -:> (gt#"Eq" • t#0)) ,
@@ -99,6 +103,14 @@ def t1 : Term := (((g#"eq@Maybe" •[gt#"Bool"]) •(.open) ((g#"EqBool" •[gt#
 -- #eval (((g#"EqBool" •[gt#"Bool"]) • refl! gt#"Bool")).infer_type MaybeBoolCtx [] []
 -- #eval ((g#"eq@Maybe" •[gt#"Bool"]) •(.open) ((g#"EqBool" •[gt#"Bool"]) • refl! gt#"Bool")).infer_type MaybeBoolCtx [] []
 
+def t := ((((g#"eq@Maybe" •[gt#"Bool"])
+       •(.open) ((g#"EqBool" •[gt#"Bool"]) • refl! gt#"Bool"))
+       • (g#"Just" •[gt#"Bool"] • g#"True")))
+       • (g#"Just" •[gt#"Bool"] • g#"True")
+
+#guard t.eval_loop MaybeBoolCtx == g#"True"
+
+
 
 -- eq : ∀ t -> Eq t -> t -> t -> Bool
 def t2 := let eqt := ((((g#"EqMaybe") •[ gt#"Maybe" • gt#"Bool" ]) •[ gt#"Bool" ])
@@ -109,73 +121,73 @@ def t2 := let eqt := ((((g#"EqMaybe") •[ gt#"Maybe" • gt#"Bool" ]) •[ gt#"
                      • ((g#"Just" •[gt#"Bool"]) • g#"True")))
                      • ((g#"Just" •[gt#"Bool"]) • g#"True")
 
--- #eval! eval_loop MaybeBoolCtx t2
+#guard t2.eval_loop MaybeBoolCtx == g#"True"
 
--- def t3 := let eqt := ((((g#"EqMaybe") •[ gt#"Maybe" • gt#"Bool" ]) •[ gt#"Bool" ])
---                                        • (refl! (gt#"Maybe" • gt#"Bool")))
---                                        • (((g#"EqBool" •[gt#"Bool"]) • refl! gt#"Bool"));
---           ((((g#"eq" •[ gt#"Maybe" • gt#"Bool" ])
---                      • eqt)
---                      • ((g#"Just" •[gt#"Bool"]) • g#"True")))
---                      • ((g#"Nothing" •[gt#"Bool"]))
+def t3 := let eqt := ((((g#"EqMaybe") •[ gt#"Maybe" • gt#"Bool" ]) •[ gt#"Bool" ])
+                                       • (refl! (gt#"Maybe" • gt#"Bool")))
+                                       • (((g#"EqBool" •[gt#"Bool"]) • refl! gt#"Bool"));
+          ((((g#"eq" •[ gt#"Maybe" • gt#"Bool" ])
+                     • eqt)
+                     • ((g#"Just" •[gt#"Bool"]) • g#"True")))
+                     • ((g#"Nothing" •[gt#"Bool"]))
 
--- #eval! eval_loop MaybeBoolCtx t3
-
-
+#guard t3.eval_loop MaybeBoolCtx == g#"False"
 
 
-#eval! eval MaybeBoolCtx t2
-def t3 := Option.getD (eval MaybeBoolCtx t2) `0
-#eval! eval MaybeBoolCtx t3
-def t4 := Option.getD (eval MaybeBoolCtx t3) `0
-#eval! eval MaybeBoolCtx t4
-def t5 := Option.getD (eval MaybeBoolCtx t4) `0
-#eval! eval MaybeBoolCtx t5
-def t6 := Option.getD (eval MaybeBoolCtx t5) `0
-#eval! eval MaybeBoolCtx t6
-def t7 := Option.getD (eval MaybeBoolCtx t6) `0
-#eval! eval MaybeBoolCtx t7
-def t8 := Option.getD (eval MaybeBoolCtx t7) `0
-#eval! eval MaybeBoolCtx t8
-def t9 := Option.getD (eval MaybeBoolCtx t8) `0
-#eval! eval MaybeBoolCtx t9
-def t10 := Option.getD (eval MaybeBoolCtx t9) `0
-#eval! eval MaybeBoolCtx t10
-def t11 := Option.getD (eval MaybeBoolCtx t10) `0
-#eval! eval MaybeBoolCtx t11
-def t12 := Option.getD (eval MaybeBoolCtx t11) `0
-#eval! eval MaybeBoolCtx t12
-def t13 := Option.getD (eval MaybeBoolCtx t12) `0
-#eval! eval MaybeBoolCtx t13
-def t14 := Option.getD (eval MaybeBoolCtx t13) `0
-#eval! eval MaybeBoolCtx t14
-def t15 := Option.getD (eval MaybeBoolCtx t14) `0
-#eval! eval MaybeBoolCtx t15
-def t16 := Option.getD (eval MaybeBoolCtx t15) `0
-#eval! eval MaybeBoolCtx t16
-def t17 := Option.getD (eval MaybeBoolCtx t16) `0
-#eval! eval MaybeBoolCtx t17
-def t18 := Option.getD (eval MaybeBoolCtx t17) `0
-#eval! eval MaybeBoolCtx t18
-def t19 := Option.getD (eval MaybeBoolCtx t18) `0
-#eval! eval MaybeBoolCtx t19
-def t20 := Option.getD (eval MaybeBoolCtx t19) `0
-#eval! eval MaybeBoolCtx t19
-def t21 := Option.getD (eval MaybeBoolCtx t20) `0
-#eval! eval MaybeBoolCtx t20
-def t22 := Option.getD (eval MaybeBoolCtx t21) `0
-#eval! eval MaybeBoolCtx t22
-def t23 := Option.getD (eval MaybeBoolCtx t22) `0
-#eval! eval MaybeBoolCtx t23
-def t24 := Option.getD (eval MaybeBoolCtx t23) `0
-#eval! eval MaybeBoolCtx t24
-def t25 := Option.getD (eval MaybeBoolCtx t24) `0
-#eval! eval MaybeBoolCtx t25
-def t26 := Option.getD (eval MaybeBoolCtx t25) `0
-#eval! eval MaybeBoolCtx t26
-def t27 := Option.getD (eval MaybeBoolCtx t26) `0
-#eval! eval MaybeBoolCtx t27
-def t28 := Option.getD (eval MaybeBoolCtx t27) `0
-#eval! eval MaybeBoolCtx t28
-def t29 := Option.getD (eval MaybeBoolCtx t28) `0
-#eval! eval MaybeBoolCtx t29
+
+
+-- #eval! eval MaybeBoolCtx t
+-- def t3 := Option.getD (eval MaybeBoolCtx t2) `0
+-- #eval! eval MaybeBoolCtx t3
+-- def t4 := Option.getD (eval MaybeBoolCtx t3) `0
+-- #eval! eval MaybeBoolCtx t4
+-- def t5 := Option.getD (eval MaybeBoolCtx t4) `0
+-- #eval! eval MaybeBoolCtx t5
+-- def t6 := Option.getD (eval MaybeBoolCtx t5) `0
+-- #eval! eval MaybeBoolCtx t6
+-- def t7 := Option.getD (eval MaybeBoolCtx t6) `0
+-- #eval! eval MaybeBoolCtx t7
+-- def t8 := Option.getD (eval MaybeBoolCtx t7) `0
+-- #eval! eval MaybeBoolCtx t8
+-- def t9 := Option.getD (eval MaybeBoolCtx t8) `0
+-- #eval! eval MaybeBoolCtx t9
+-- def t10 := Option.getD (eval MaybeBoolCtx t9) `0
+-- #eval! eval MaybeBoolCtx t10
+-- def t11 := Option.getD (eval MaybeBoolCtx t10) `0
+-- #eval! eval MaybeBoolCtx t11
+-- def t12 := Option.getD (eval MaybeBoolCtx t11) `0
+-- #eval! eval MaybeBoolCtx t12
+-- def t13 := Option.getD (eval MaybeBoolCtx t12) `0
+-- #eval! eval MaybeBoolCtx t13
+-- def t14 := Option.getD (eval MaybeBoolCtx t13) `0
+-- #eval! eval MaybeBoolCtx t14
+-- def t15 := Option.getD (eval MaybeBoolCtx t14) `0
+-- #eval! eval MaybeBoolCtx t15
+-- def t16 := Option.getD (eval MaybeBoolCtx t15) `0
+-- #eval! eval MaybeBoolCtx t16
+-- def t17 := Option.getD (eval MaybeBoolCtx t16) `0
+-- #eval! eval MaybeBoolCtx t17
+-- def t18 := Option.getD (eval MaybeBoolCtx t17) `0
+-- #eval! eval MaybeBoolCtx t18
+-- def t19 := Option.getD (eval MaybeBoolCtx t18) `0
+-- #eval! eval MaybeBoolCtx t19
+-- def t20 := Option.getD (eval MaybeBoolCtx t19) `0
+-- #eval! eval MaybeBoolCtx t19
+-- def t21 := Option.getD (eval MaybeBoolCtx t20) `0
+-- #eval! eval MaybeBoolCtx t20
+-- def t22 := Option.getD (eval MaybeBoolCtx t21) `0
+-- #eval! eval MaybeBoolCtx t22
+-- def t23 := Option.getD (eval MaybeBoolCtx t22) `0
+-- #eval! eval MaybeBoolCtx t23
+-- def t24 := Option.getD (eval MaybeBoolCtx t23) `0
+-- #eval! eval MaybeBoolCtx t24
+-- def t25 := Option.getD (eval MaybeBoolCtx t24) `0
+-- #eval! eval MaybeBoolCtx t25
+-- def t26 := Option.getD (eval MaybeBoolCtx t25) `0
+-- #eval! eval MaybeBoolCtx t26
+-- def t27 := Option.getD (eval MaybeBoolCtx t26) `0
+-- #eval! eval MaybeBoolCtx t27
+-- def t28 := Option.getD (eval MaybeBoolCtx t27) `0
+-- #eval! eval MaybeBoolCtx t28
+-- def t29 := Option.getD (eval MaybeBoolCtx t28) `0
+-- #eval! eval MaybeBoolCtx t29
