Core/Term/Definition.lean
@@ -36,7 +36,7 @@ inductive Term : Type where
 | tbind : TyBindVariant -> Kind -> Term -> Term
 | lam : Ty -> Term -> Term
 | guard : Term -> Term -> Term -> Term
-| «match» : Term -> Vec Term n -> Vec Term n -> Term
+| «match» : Term -> Vec Term n -> Vec Term n -> Term -> Term
 
 prefix:max "#" => Term.var
 prefix:max "g#" => Term.global
@@ -79,7 +79,7 @@ def Term.size : Term -> Nat
 | tbind _ _ t => size t + 1
 | lam _ t => size t + 1
 | guard t1 t2 t3 => size t1 + size t2 + size t3 + 1
-| .match t1 t2 t3 => size t1 + Vec.sum (λ i => (t2 i).size) + Vec.sum (λ i => (t3 i).size) + 1
+| .match t1 t2 t3 t4 => size t1 + Vec.sum (λ i => (t2 i).size) + Vec.sum (λ i => (t3 i).size) + size t4 + 1
 
 @[simp]
 instance instSizeOf_Term : SizeOf Term where
@@ -118,13 +118,16 @@ protected def Term.repr (p : Nat) : (a : Term) -> Std.Format
 | .tbind .allc K t =>
   Repr.addAppParen ("∀c" ++ Std.Format.sbracket (repr K) ++ " " ++ Term.repr max_prec t) p
 | .lam τ t => Repr.addAppParen ("λ" ++ Std.Format.sbracket (repr τ) ++ " " ++ Term.repr max_prec t) p
-| .match (n := n) s pats ts =>
+| .match (n := n) s pats ts allc =>
   let ts : Vec Std.Format n := λ i =>
     let t := ts i
     let pat := pats i
     Std.Format.nest 4 <| Std.Format.line ++ Term.repr p pat ++ " => " ++ Term.repr p t
-  Std.Format.nest 4 <| ("match " ++ Term.repr p s)
-    ++ Vec.fold (·++·) Std.Format.nil ts
+  let css := Vec.fold (·++·) Std.Format.nil ts
+  Std.Format.nest 4 <| (("match " ++ Term.repr p s ++ "with")
+    ++ css
+    ++ (Std.Format.nest 4 <| Std.Format.line ++ " _ => " ++ Term.repr p allc)
+    )
 | .guard pat s t =>
   Std.Format.nest 4 <| ("guard " ++ Term.repr p pat ++ " ← " ++ Term.repr p s) ++
   Std.Format.line ++ Term.repr p t
