Core/Examples/FunDeps.lean
@@ -3,7 +3,7 @@ import Core.Term
 import Core.Global
 import Core.Vec
 
-import Core.Eval.BigStep
+import Core.Infer.Global
 
 def FunDepsCtx : List Global := [
 
@@ -11,8 +11,9 @@ def FunDepsCtx : List Global := [
   --     Λ A B. λ i a. a |> fdEqual1 A A B (EqualTT A A (refl A)) i
   .defn "id" (∀[★]∀[★] ((gt#"Equal" • t#1) • t#0) -:> t#1 -:> t#0) (
     Λ[★]Λ[★] λ[((gt#"Equal" • t#1) • t#0) ] λ[t#1]
-      (#0 ▹ ((((g#"fdFwd" •[t#1]) •[t#1]) • (((g#"EqualTT" •[t#1]) •[t#1]) • (refl! t#1))) • #1))
+      (#0 ▹ (((((g#"fdFwd" •[t#1]) •[t#1]) •[t#0]) •(.open) (((g#"EqualTT" •[t#1]) •[t#1]) • (refl! t#1))) •(.open) #1))
   ),
+
   -- instance fdEqual2 = Λ t t' u. λ i1 i2.
   --     guard EqualTT[t, u] <- i1 then λ c1.
   --     guard EqualTT[t', u] <- i2 then λ c2.
@@ -24,26 +25,27 @@ def FunDepsCtx : List Global := [
     )
   ),
 
-  -- instance fdEqual1 = Λ t u u'. λ i1 i2.
-  --     guard EqualTT[t, u] <- i1 then λ c1.
-  --     guard EqualTT[t, u'] <- i2 then λ c2.
+  -- instance fdEqual1 = Λ t u u'. λ i1 i0.
+  --     guard EqualTT[t, u] <- i1 then λ c1 : t ~ u.
+  --     guard EqualTT[t, u'] <- i0 then λ c2 : t ~ u'.
   --         sym c1 ; c2
   .inst "fdFwd" (Λ[★]Λ[★]Λ[★] λ[(gt#"Equal" • t#2) • t#1] λ[(gt#"Equal" • t#2) • t#0 ]
     .guard ((g#"EqualTT" •[t#2]) •[t#1]) #1 (λ[t#2 ~[★]~ t#1]
       .guard ((g#"EqualTT" •[t#2]) •[t#0]) #1 (λ[t#2 ~[★]~ t#0]
-            sym! #1 `; #0)
+            (sym! #1 `; #0))
     )
   ),
 
-
   -- instance EqualTT :: ∀ t u. t ~ u -> Equal t u
-  .instty "EqualTT" (∀[★]∀[★] t#1 ~[★]~ t#0 -:> ((gt#"Equal" • t#1) • t#0)),
+  .instty "EqualTT" (∀[★]∀[★] (t#1 ~[★]~ t#0) -:> ((gt#"Equal" • t#1) • t#0)),
 
   -- open fdBwk :: ∀ t t' u. Equal t u -> Equal t' u -> t ~ t'
-  .openm "fdFwd" (∀[★] ∀[★] ∀[★] ((gt#"Equal" • t#2) • t#0) -:>  ((gt#"Equal" • t#1) • t#0) -:> (t#2 ~[★]~ t#1)),
+  .openm "fdBwk" (∀[★] ∀[★] ∀[★] ((gt#"Equal" • t#2) • t#0) -:>  ((gt#"Equal" • t#1) • t#0) -:> (t#2 ~[★]~ t#1)),
   -- open fdFwd :: ∀ t u u'. Equal t u -> Equal t u' -> u ~ u'
   .openm "fdFwd" (∀[★] ∀[★] ∀[★] ((gt#"Equal" • t#2) • t#1) -:>  ((gt#"Equal" • t#2) • t#0) -:> (t#1 ~[★]~ t#0)),
 
   .opent "Equal" (★ -:> ★ -:> ◯)
 
 ]
+
+#guard Globals.wf_globals FunDepsCtx == .some ()
